updates final commit

Sources/ConversionToBoogie/AST_Handler.cs
@@ -1,0 +1,455 @@
+﻿
+
+namespace ConversionToBoogie
+{
+    using System;
+    using System.Collections.Generic;
+    using System.Diagnostics;
+    using System.Linq;
+    using Boogie_Syntax_Tree;
+    using Sol_Syntax_Tree;
+
+    /**
+     * ASTHandler class to act as filtration for solidity AST properties
+     */
+    public class AST_Handler
+    {
+        public static int MAX_GAS_LIMIT = 7000000;
+        public static int MIN_GAS_LIMIT = 3000000;
+
+        //return 
+        public BoogieProgram getProgram { get; private set; }
+
+        public Dictionary<int, ASTNode> IdToNodeMap { get; set; }
+
+        public string SourceDirectory { get; set; }
+
+        // source file path of ASTNode
+        public Dictionary<ASTNode, string> ASTNodeToSourcePathMap { get; private set; }
+
+        // source file line number of ASTNode
+        public Dictionary<ASTNode, int> ASTLineNumberMap { get; private set; }
+
+        // all contracts defined in the program
+        public HashSet<ContractDefinition> ContractDefinitionsMap { get; private set; }
+
+        // map from each contract to its sub types (including itself)
+        public Dictionary<ContractDefinition, HashSet<ContractDefinition>> SubTypeMapping { get; private set; }
+
+        // all state variables explicitly defined in each contract
+        public Dictionary<ContractDefinition, HashSet<VariableDeclaration>> StateVarMaps { get; private set; }
+        public Dictionary<VariableDeclaration, ContractDefinition> StateVarToContractMap { get; private set; }
+
+        // all mappings explicitly defined in each contract
+        public Dictionary<ContractDefinition, HashSet<VariableDeclaration>> MappingFrame { get; private set; }
+        // all arrays explicityly defined in each contract
+        public Dictionary<ContractDefinition, HashSet<VariableDeclaration>> constructArrayMaps { get; private set; }
+
+        // explicit constructor defined in each contract
+        // solidity only allows at most one constructor for each contract
+        public Dictionary<ContractDefinition, FunctionDefinition> ConstructorMapping { get; private set; }
+
+        // explicit fallback defined in each contract
+        // solidity only allows at most one fallback for each contract
+        public Dictionary<ContractDefinition, FunctionDefinition> FallbackMap { get; private set; }
+
+        // all events explicitly defined in each contract
+        public Dictionary<ContractDefinition, HashSet<EventDefinition>> EventMapping { get; private set; }
+        public Dictionary<EventDefinition, ContractDefinition> EventToContractMap { get; private set; }
+
+        // all functions explicitly defined in each contract
+        // FIXME: getters for public state variables
+        public Dictionary<ContractDefinition, HashSet<FunctionDefinition>> FunctionMapping { get; private set; }
+        public Dictionary<ContractDefinition, HashSet<string>> FunctionSignatureMapping { get; private set; }
+        public Dictionary<FunctionDefinition, ContractDefinition> FunctionToContractMap { get; private set; }
+
+        // FunctionSignature -> (DynamicType -> FunctionDefinition)
+        public Dictionary<string, Dictionary<ContractDefinition, FunctionDefinition>> SignatureFunctionMap { get; private set; }
+        // all functions (including private ones) visible in each contract
+        public Dictionary<ContractDefinition, HashSet<FunctionDefinition>> FunctionsMap { get; private set; }
+
+        // StateVarName -> (Dynamictype -> StateVariableDeclaration)
+        public Dictionary<string, Dictionary<ContractDefinition, VariableDeclaration>> stateVarLookUpTable { get; private set; }
+        // all state variables (including private ones) visible in each contract
+        public Dictionary<ContractDefinition, HashSet<VariableDeclaration>> VisibleStateMapping { get; private set; }
+
+
+        public Dictionary<string, BoogieImplementation> ModifierToBoogiePreImpl { get; private set;}
+
+        public Dictionary<string, BoogieImplementation> ModifierToBoogiePostImpl { get; private set;}
+
+        // Options flags, currently not in use
+        public Flags_HelperClass TranslateFlags { get; private set; }
+
+        public Dictionary<ContractDefinition, Dictionary<UserDefinedTypeName, TypeName>> constructDefinitionsMap => usingMap;
+
+        // num of fresh identifiers, should be incremented when making new fresh id
+        private int indentifierCount = 0;
+
+        // methods whose translation has to be skipped, 
+        private readonly HashSet<Tuple<string, string>> IgnoreMethods;
+
+        private readonly bool genInlineAttrInBpl;
+
+        // data structures for using
+        // maps Contract C --> (source, dest), where source is a library type
+        private Dictionary<ContractDefinition, Dictionary<UserDefinedTypeName, TypeName>> usingMap;
+
+        //ignored methods and translate flags not used, intended for implementation however timeconstraints prohibited this.
+        //Parameter based constructor.
+        public AST_Handler(HashSet<Tuple<string, string>> ignoreMethods, bool _genInlineAttrInBpl, Flags_HelperClass translateFlags = null)
+        {
+
+            //returns boogie program instance containing the building blocks for boogie statements.
+            //Initially this property is populated with default Boogie Statements as per expectation of the Boogie veriifer.
+
+            //The process handler then aids in conversion to boogie by providing Boogie alternatives to the soldiity constructs contained within each mapping.
+            getProgram = new BoogieProgram();
+            //generates the mappings for the AST_hander, used to filter the generic AST properties into categorizable subsections
+            instantiateMappings();
+
+            IgnoreMethods = ignoreMethods;
+            genInlineAttrInBpl = _genInlineAttrInBpl; // set by default to true;
+            TranslateFlags = translateFlags;//Not used
+        }
+        /**
+         * function check whether an id contains an ast node at the given index
+         */
+        public bool HasASTNodeId(int id)
+        {
+            return IdToNodeMap.ContainsKey(id);
+        }
+
+        // function to retrieve an ASTNode instance given an id
+        public ASTNode retrieveASTNodethroughID(int id)
+        {
+            if (IdToNodeMap.ContainsKey(id))
+            {
+                return IdToNodeMap[id];
+            }
+            else
+            {
+                return null;
+            }
+        }
+        // function to add source info to ast node
+        public void AddSourceInfoForASTNode(ASTNode node, string absolutePath, int lineNumber)
+        {
+            Debug.Assert(!ASTNodeToSourcePathMap.ContainsKey(node));
+            Debug.Assert(!ASTLineNumberMap.ContainsKey(node));
+            ASTNodeToSourcePathMap[node] = absolutePath;
+            ASTLineNumberMap[node] = lineNumber;
+        }
+        /**
+         * Return absolute path of ast node, given the node instance
+         */
+        public string GetAbsoluteSourcePathOfASTNode(ASTNode node)
+        {
+            return ASTNodeToSourcePathMap[node];
+        }
+        /**
+         * Return line number of ast node, given node
+         */
+        public int GetLineNumberOfASTNode(ASTNode node)
+        {
+            return ASTLineNumberMap[node];
+        }
+        /**
+         * retrieve function defintions using contract as an identifier to traverse the FunctionMapping.
+         */
+        public HashSet<FunctionDefinition> returnFunctionDefs(ContractDefinition contract)
+        {
+            if (FunctionMapping.ContainsKey(contract))
+            {
+                return FunctionMapping[contract];
+            }
+            return new HashSet<FunctionDefinition>();
+        }
+        //Return Event Defintions using Contract as an indentifier to traverse the Event mapping.
+        public HashSet<EventDefinition> retrieveEventDefinitionsUsingContract(ContractDefinition contract)
+        {
+            if (EventMapping.ContainsKey(contract))
+            {
+                return EventMapping[contract];
+            }
+            else
+            {
+                return new HashSet<EventDefinition>();
+            }
+        }
+
+        //Insert contract into contract defintiions collection.
+        public void InsertContractInMapping(ContractDefinition contract)
+        {
+            ContractDefinitionsMap.Add(contract);
+        }
+
+        /**
+         * Return the contract name from a collection of contracts (using identifier) 
+         */
+        public ContractDefinition retrieveContractName(string contractName)
+        {
+            foreach (ContractDefinition contract in ContractDefinitionsMap)
+            {
+                if (contract.Name.Equals(contractName))
+                {
+                    return contract;
+                }
+            }
+            return null;
+        }
+
+        //Insert SubTypeMapping to contract parameter.
+        public void InsertTypeInContract(ContractDefinition contract, ContractDefinition type)
+        {
+            if (SubTypeMapping.ContainsKey(contract) == false)
+            {
+                SubTypeMapping[contract] = new HashSet<ContractDefinition>();
+            }
+            SubTypeMapping[contract].Add(type);
+        }
+
+        //Function to return sub types for a specific contract through indexing it in the collections map
+        public HashSet<ContractDefinition> returnSubTypesIndex(ContractDefinition contract)
+        {
+            return SubTypeMapping[contract];
+        }
+
+        public void AddStateVarToContract(ContractDefinition contract, VariableDeclaration Declaration)
+        {
+            //check whether collection does not already contain the new addition 
+            //if not then create a new hashset with the proposed contract and place it into the collection
+            if (StateVarMaps.ContainsKey(contract) == false)
+            {
+                StateVarMaps[contract] = new HashSet<VariableDeclaration>();
+            }
+
+            //add the node to the indexed contract within the collection
+            StateVarMaps[contract].Add(Declaration);
+            //assign statevar collections map with the index of varDec1 the value of the given contract
+            StateVarToContractMap[Declaration] = contract;
+        }
+
+        //Insert Mapping declaration into contract using 
+        public void InsertMappingInContract(ContractDefinition contract, VariableDeclaration mappingDeclaration)
+        {
+            if (MappingFrame.ContainsKey(contract) == false)
+            {
+                MappingFrame[contract] = new HashSet<VariableDeclaration>();
+            }
+            MappingFrame[contract].Add(mappingDeclaration);
+        }
+
+        //Insert Array into contract using ArrayMapping.
+        public void insertArrayInContract(ContractDefinition contract, VariableDeclaration array)
+        {
+            if (constructArrayMaps.ContainsKey(contract) == false)
+            {
+                constructArrayMaps[contract] = new HashSet<VariableDeclaration>();
+            }
+            constructArrayMaps[contract].Add(array);
+        }
+
+        //Retrieve state variables through contract 
+        public HashSet<VariableDeclaration> retrieveStateVariables(ContractDefinition contract)
+        {
+            bool containsKey = StateVarMaps.ContainsKey(contract);
+
+            if (containsKey){
+                return StateVarMaps[contract];
+            }
+            else
+            {
+                new HashSet<VariableDeclaration>();
+            }
+            return null;
+        }
+
+        //Insert constructor into contract using constructor mapping
+        public void InsertConstructorInContract(ContractDefinition contract, FunctionDefinition ctor)
+        {
+            ConstructorMapping[contract] = ctor;
+        }
+
+        //Function to insert fallback definition to contract using fallback mapping
+        public void InsertFallBackInContract(ContractDefinition contract, FunctionDefinition fallback)
+        {
+            FallbackMap[contract] = fallback;
+        }
+
+        //Function to check if constructor exists.
+        public bool checkConstructorExists(ContractDefinition contract)
+        {
+            bool contains = ConstructorMapping.ContainsKey(contract);
+
+            return contains;
+        }
+
+        //Function to retrieve constructor from ConstructorMap
+        public FunctionDefinition retrieveConstructor(ContractDefinition contract)
+        {
+            if (ConstructorMapping.ContainsKey(contract))
+            {
+                return ConstructorMapping[contract];
+            }
+            return null;
+        }
+
+        //Function to insert an event into the argument contract.
+        public void InsertEventInContract(ContractDefinition contract, EventDefinition eventDef)
+        {
+            //if the event map does not contain the contract, then add it
+            //if the eventMap does not contain the event definition, then add it.
+            if (EventMapping.ContainsKey(contract) == false)
+            {
+                EventMapping[contract] = new HashSet<EventDefinition>();
+            }
+
+            if (EventMapping[contract].Contains(eventDef) == false)
+            {
+                EventMapping[contract].Add(eventDef);
+            }
+        }
+
+        //function to check whether an event name is contain in a contract.
+        public bool containsEventName(ContractDefinition contract, string eventName)
+        {
+            if (!EventMapping.ContainsKey(contract))
+            {
+                return false;
+            }
+            foreach (EventDefinition eventDef in EventMapping[contract])
+            {
+                if (eventName.Equals(eventDef.Name))
+                {
+                    return true;
+                }
+            }
+            return false;
+        }
+
+        //Function to insert a function into the specified contract.
+        public void InsertFunctionInContract(ContractDefinition contract, FunctionDefinition funcDef)
+        {
+            if (FunctionMapping.ContainsKey(contract) == false)
+            {
+                Debug.Assert(!FunctionSignatureMapping.ContainsKey(contract));
+                FunctionMapping[contract] = new HashSet<FunctionDefinition>();
+                FunctionSignatureMapping[contract] = new HashSet<string>();
+            }
+
+            Debug.Assert(!FunctionMapping[contract].Contains(funcDef), $"Repeated function warning: {funcDef.Name}");
+            FunctionMapping[contract].Add(funcDef);
+
+            string signature = Conversion_Utility_Tool.ComputeFunctionSignature(funcDef);
+            FunctionSignatureMapping[contract].Add(signature);
+
+            Debug.Assert(!FunctionToContractMap.ContainsKey(funcDef), $" Repeated function warning: {funcDef.Name}");
+            FunctionToContractMap[funcDef] = contract;
+        }
+
+        public ContractDefinition GetContractByFunction(FunctionDefinition funcDef)
+        {
+            Debug.Assert(FunctionToContractMap.ContainsKey(funcDef));
+            return FunctionToContractMap[funcDef];
+        }
+
+
+        public void AddFunctionToDynamicType(string funcSig, ContractDefinition dynamicType, FunctionDefinition funcDef)
+        {
+            if (!SignatureFunctionMap.ContainsKey(funcSig))
+            {
+                SignatureFunctionMap[funcSig] = new Dictionary<ContractDefinition, FunctionDefinition>();
+            }
+
+            // may potentially override the previous value due to inheritance
+            SignatureFunctionMap[funcSig][dynamicType] = funcDef;
+        }
+
+        public bool doesContainFunctionSignature(string funcSig)
+        {
+            return SignatureFunctionMap.ContainsKey(funcSig);
+        }
+
+        //Function to return definitions.
+        public Dictionary<ContractDefinition, FunctionDefinition> returnFunctionDefintiions(string functionSignature)
+        {
+            return SignatureFunctionMap[functionSignature];
+        }
+
+        public void AddVisibleFunctionToContract(FunctionDefinition funcDef, ContractDefinition contract)
+        {
+            if (FunctionsMap.ContainsKey(contract) == false)
+            {
+                FunctionsMap[contract] = new HashSet<FunctionDefinition>();
+            }
+            else
+            {
+                //do nothing
+            }
+            FunctionsMap[contract].Add(funcDef);
+        }
+
+
+        //Function to return a hashset of functiondefinitions that are retrieved using a contract instance.
+        public HashSet<FunctionDefinition> RetrieveVisibleFunctions(ContractDefinition contract)
+        {
+            if (FunctionsMap.ContainsKey(contract)){
+                return FunctionsMap[contract];
+            }
+            else
+            {
+                new HashSet<FunctionDefinition>();
+            }
+            //should not reutnr null, but there lies a possiblity
+            return null;
+        }
+
+
+
+        //Function to check whether conditional contains statevar
+        public bool ContainsStateVar(string varName)
+        {
+            return stateVarLookUpTable.ContainsKey(varName);
+        }
+
+        //returns state variable using lookup map with an index of dynamic type
+        public VariableDeclaration retrieveStateVarDynamicType(string variableName, ContractDefinition dynamicType)
+        {
+            return stateVarLookUpTable[variableName][dynamicType];
+        }
+
+        //generate fresh identifier using BoogieType
+        public BoogieTypedIdent createFreshIdentifier(BoogieType type)
+        {
+            //return new BoogieTypedIdent.
+            string name = "__var_" + indentifierCount;
+            return new BoogieTypedIdent(name, type);
+        }
+
+        private void instantiateMappings()
+        {
+            ContractDefinitionsMap = new HashSet<ContractDefinition>();
+            ASTNodeToSourcePathMap = new Dictionary<ASTNode, string>();
+            ASTLineNumberMap = new Dictionary<ASTNode, int>();
+            SubTypeMapping = new Dictionary<ContractDefinition, HashSet<ContractDefinition>>();
+            StateVarMaps = new Dictionary<ContractDefinition, HashSet<VariableDeclaration>>();
+            MappingFrame = new Dictionary<ContractDefinition, HashSet<VariableDeclaration>>();
+            constructArrayMaps = new Dictionary<ContractDefinition, HashSet<VariableDeclaration>>();
+            StateVarToContractMap = new Dictionary<VariableDeclaration, ContractDefinition>();
+            ConstructorMapping = new Dictionary<ContractDefinition, FunctionDefinition>();
+            FallbackMap = new Dictionary<ContractDefinition, FunctionDefinition>();
+            EventMapping = new Dictionary<ContractDefinition, HashSet<EventDefinition>>();
+            EventToContractMap = new Dictionary<EventDefinition, ContractDefinition>();
+            FunctionMapping = new Dictionary<ContractDefinition, HashSet<FunctionDefinition>>();
+            FunctionSignatureMapping = new Dictionary<ContractDefinition, HashSet<string>>();
+            FunctionToContractMap = new Dictionary<FunctionDefinition, ContractDefinition>();
+            SignatureFunctionMap = new Dictionary<string, Dictionary<ContractDefinition, FunctionDefinition>>();
+            FunctionsMap = new Dictionary<ContractDefinition, HashSet<FunctionDefinition>>();
+            stateVarLookUpTable = new Dictionary<string, Dictionary<ContractDefinition, VariableDeclaration>>();
+            VisibleStateMapping = new Dictionary<ContractDefinition, HashSet<VariableDeclaration>>();
+            usingMap = new Dictionary<ContractDefinition, Dictionary<UserDefinedTypeName, TypeName>>();
+        }
+
+    }
+}
