Sources/ConversionToBoogie/ConversionToBoogie_Main.cs
@@ -1,0 +1,172 @@
+
+
+namespace ConversionToBoogie
+{
+    using System;
+    using System.Collections.Generic;
+    using System.Diagnostics;
+    using Boogie_Syntax_Tree;
+    using Sol_Syntax_Tree;
+
+    //Dedicated class to handle conversion from solidity AST to Boogie AST such that the verification power of Boogie.exe can be leveraged.
+
+    public class ConversionToBoogie_Main
+    {
+        // set of method@contract pairs whose translation is skipped
+
+        SourceUnitList sourceUnits = null;
+        AST_Handler classTranslatorContext;
+
+        OverSight_ProcessHandler processHandler;
+
+        //returns a boogieAST reference, containing all captured elements of the sol file in question
+        public BoogieAST Translate(AST solidityAST, HashSet<Tuple<string, string>> ignoredMethods, Flags_HelperClass _translatorFlags = null)
+        {
+            //ignored methods and translator flags need to be remove as not enough time to implement these.
+
+            sourceUnits = solidityAST.GetSourceUnits();
+
+            //create an empty AST_Handler Instance with no ignored method, generate InlineAttributes and no translator flags.
+            AST_Handler context = new AST_Handler(ignoredMethods, true, _translatorFlags);
+            context.IdToNodeMap = solidityAST.GetIdToNodeMap();
+            context.SourceDirectory = solidityAST.SourceDirectory;
+
+            //assign class instance to temporary instance and use it throughout the rest of the
+            //process to populate it.
+            classTranslatorContext = context;
+
+            //Execute Collection process from given sol contract.
+            //Will enable boogie conversion to occur once specific states/functions/variables have been retrieved from the contract.
+            executeSourceInfoCollector();
+            executeContractCollection();
+           
+            executeInheritanceCollector();
+            executeStateVariableCollector();
+            executeMapArrayCollector();
+            executeConstructorCollector();
+            
+            executeFunctionEventCollector();
+            executeFunctionEventResolver();
+
+            executeBoogieGenerator();
+            executeDefinitionsCollector();
+
+            executeProcessHandler();
+            // generate harness for contract
+            // non specifiable property, harness is always created and cannot be altered in this code
+            OverSight_Harness_Generator harnessGenerator = new OverSight_Harness_Generator();
+            harnessGenerator.setTranslatorContext(classTranslatorContext);
+            harnessGenerator.createHarness();
+            
+
+            BoogieAST completeAST = new BoogieAST(classTranslatorContext.getProgram);
+
+            Debug.Assert(completeAST != null);
+            
+            //returns the BoogieAST containing the root property, where the declarations of the contract are present.
+            return completeAST;
+        }
+
+    //Function to collect source info
+    private void executeSourceInfoCollector()
+    {
+        // collect the absolute source path and line number for each AST node
+        accumulator_SOL_srcInfo sourceInfoCollector = new accumulator_SOL_srcInfo();
+        sourceInfoCollector.setContext(classTranslatorContext);
+        sourceUnits.Accept(sourceInfoCollector);
+
+    }
+
+    //function to collect contracts.
+    private void executeContractCollection()
+    {
+        // collect all contract definitions
+        accumulator_SOL_Contract contractCollector = new accumulator_SOL_Contract();
+        contractCollector.setContext(classTranslatorContext);
+        sourceUnits.Accept(contractCollector);
+    }
+
+    //functino to collect inheritance properties
+    private void executeInheritanceCollector()
+    {
+        // collect all sub types for each contract
+        accumulator_SOL_Inheritance inheritanceCollector = new accumulator_SOL_Inheritance();
+        inheritanceCollector.setContext(classTranslatorContext);
+        inheritanceCollector.checkContractForInheritance();
+    }
+
+    //function to collect statevariables
+    private void executeStateVariableCollector()
+    {
+        // collect explicit state variables
+        accumulator_SOL_StateVariable stateVariableCollector = new accumulator_SOL_StateVariable();
+        stateVariableCollector.setContext(classTranslatorContext);
+        sourceUnits.Accept(stateVariableCollector);
+    }
+
+    //function to collect maps and arrays
+    private void executeMapArrayCollector()
+    {
+        // collect mappings and arrays
+        accumulator_SOL_Map_Arrays mapArrayCollector = new accumulator_SOL_Map_Arrays();
+        mapArrayCollector.setContext(classTranslatorContext);
+        sourceUnits.Accept(mapArrayCollector);
+    }
+
+    //function to collect constructor
+    private void executeConstructorCollector()
+    {
+        // collect constructor definitions
+        accumulator_SOL_Constructor constructorCollector = new accumulator_SOL_Constructor();
+        constructorCollector.setContext(classTranslatorContext);
+        sourceUnits.Accept(constructorCollector);
+    }
+
+    //function to collect functions and events 
+    private void executeFunctionEventCollector()
+    {
+        // collect explicit function and event definitions
+        accumulator_SOL_Functions_Events functionEventCollector = new accumulator_SOL_Functions_Events();
+        functionEventCollector.setContext(classTranslatorContext);
+        sourceUnits.Accept(functionEventCollector);
+    }
+
+    /**
+     * Function to resolve solidity functions and events to boogie
+     */
+    private void executeFunctionEventResolver()
+    {
+        // resolve function and event definitions and determine the actual definition for a dynamic type
+        OverSight_Function_Event_Resolver functionEventResolver = new OverSight_Function_Event_Resolver();
+        functionEventResolver.setTranslatorContext(classTranslatorContext);
+        functionEventResolver.filterFunctionsAndEvents();      
+    }
+
+    /**
+     * Function to generate boogie properties, including maps, type, global implementations and so forth
+     */
+    private void executeBoogieGenerator()
+    {
+        OverSight_Boogie_Generate_Properties generator = new OverSight_Boogie_Generate_Properties(classTranslatorContext);
+        generator.GenerateBoogieProperties();
+    }
+
+    /**
+     * Function to collect definitions from soldity AST and parse to Boogie
+     */
+    private void executeDefinitionsCollector()
+    {
+        // collect all using definitions
+        DefinitionsAccumulator usingCollector = new DefinitionsAccumulator();
+        usingCollector.setContext(classTranslatorContext);
+        sourceUnits.Accept(usingCollector);
+    }
+    private void executeProcessHandler()
+    {
+        // start process handler and generate inlineattributes
+        OverSight_ProcessHandler procTranslator = new OverSight_ProcessHandler(classTranslatorContext, true);
+        sourceUnits.Accept(procTranslator);
+        this.processHandler = procTranslator;
+    }
+}
+}
