Sources/ConversionToBoogie/OverSight_Boogie_Generate_Properties.cs
@@ -1,0 +1,408 @@
+﻿
+
+namespace ConversionToBoogie
+{
+    using System.Collections.Generic;
+    using System.Diagnostics;
+    using Boogie_Syntax_Tree;
+    using Sol_Syntax_Tree;
+
+    /**
+     * Public Generation class for Boogie Properties 
+     * Invoked via ConversionToBoogieMain,cs
+     */
+    public class OverSight_Boogie_Generate_Properties
+    {
+        // AST_Handler context to leverage "getProgram" and updated with
+        // Boogie Types, Constants, Functions, Global Variables and Global Implementations 
+        private AST_Handler context;
+
+        public OverSight_Boogie_Generate_Properties(AST_Handler context){ this.context = context; }
+
+        //Function invoked via ConversionToBoogie_Main.cs to generate default boogie properties expected by verifier.
+        public void GenerateBoogieProperties()
+        {
+            buildTypes(); //Generate types and add to classContext.BoogieProgram
+            buildConstants(); //Generate Constants and add to classContext.BoogieProgram
+            buildFunctions(); //Generate Functions and add to classContext.BoogieProgram
+            buildGlobalVariables(); //Generate GlobalVariables and add to classContext.BoogieProgram
+            buildGlobalImplementations(); //Generate Global implementations and add to classContext.BoogieProgram
+        }
+        /**
+         * Build types and add them to Boogie Program attached to the Handler reference.
+         */
+        private void buildTypes()
+        {
+            context.getProgram.AddBoogieDeclaration(new BoogieTypeCtorDecl("Ref"));
+            context.getProgram.AddBoogieDeclaration(new BoogieTypeCtorDecl("ContractName"));
+        }
+
+        //Build functions and add them as declarations to the Boogie program located within AST_Handler
+        private void buildFunctions()
+        { 
+            context.getProgram.AddBoogieDeclaration(BuildConstantToReferenceFunction());//conversion of primitve type int to refrence type
+            context.getProgram.AddBoogieDeclaration(BuildModularFunction());//modulo operation for unsigned integers
+            context.getProgram.AddBoogieDeclaration(buildOverSightSumFunction());//Used for creation of summaping in specification as Boogie Function
+        }
+
+        /**
+        * Function to handle global implementation generation
+        */
+        private void buildGlobalImplementations()
+        {
+            BuildGlobalProcedureFresh();
+            GenerateGlobalProcedureAllocMany();
+            BuildBoogieRecordType("int", BoogieType.Int);
+            BuildBoogieRecordType("ref", BoogieType.Ref);
+            BuildBoogieRecordType("bool", BoogieType.Bool);
+            buildStructConstructor();
+        }
+
+        //Build ConstantToReferenceFunction
+        private BoogieFunction BuildConstantToReferenceFunction()
+        {
+            //function for Int to Ref
+            var inVar = new BoogieFormalParam(new BoogieTypedIdent("x", BoogieType.Int));
+            var outVar = new BoogieFormalParam(new BoogieTypedIdent("ret", BoogieType.Ref));
+            return new BoogieFunction(
+                "ConstantToRef",
+                new List<BoogieVariable>() { inVar },
+                new List<BoogieVariable>() { outVar },
+                null);
+        }
+        //Function to construct modular function call witin bpl file when leveraging the boogie verifier.
+        private BoogieFunction BuildModularFunction()
+        {
+            //function for arithmetic "modulo" operation for unsigned integers
+            string functionName = "modBpl";
+
+            var inputVariable_1 = new BoogieFormalParam(new BoogieTypedIdent("x", BoogieType.Int));
+            var inputVariable_2 = new BoogieFormalParam(new BoogieTypedIdent("y", BoogieType.Int));
+
+            var outVar = new BoogieFormalParam(new BoogieTypedIdent("ret", BoogieType.Int));
+
+            return new BoogieFunction(
+                functionName,
+                new List<BoogieVariable>() { inputVariable_1, inputVariable_2 },
+                new List<BoogieVariable>() { outVar },
+                new List<BoogieAttribute> { new BoogieAttribute("bvbuiltin", "\"" + "mod" + "\"") });
+        }
+
+        //Function to construct OverSight Sum function builder as part of the BoogieProgram.
+        private BoogieFunction buildOverSightSumFunction()
+        {
+            //function for [Ref]int to int
+            var inputVariables = new BoogieFormalParam(new BoogieTypedIdent("x", new BoogieMapType(BoogieType.Ref, BoogieType.Int)));
+            var outputVriables = new BoogieFormalParam(new BoogieTypedIdent("ret", BoogieType.Int));
+            return new BoogieFunction(
+                "_SumMapping_OverSight",
+                new List<BoogieVariable>() { inputVariables },
+                new List<BoogieVariable>() { outputVriables },
+                null);
+        }
+
+        //Function to introduce constant properties to Boogie such as REF and Constant
+        private void buildConstants()
+        {
+            BoogieConstant nullConstant = new BoogieConstant(new BoogieTypedIdent("null", BoogieType.Ref), true);
+            context.getProgram.AddBoogieDeclaration(nullConstant);
+
+            // constants for contract names
+            BoogieCtorType tnameType = new BoogieCtorType("ContractName");
+            foreach (ContractDefinition contract in context.ContractDefinitionsMap)
+            {
+                BoogieTypedIdent typedIdent = new BoogieTypedIdent(contract.Name, tnameType);
+                BoogieConstant contractNameConstant = new BoogieConstant(typedIdent, true);
+                context.getProgram.AddBoogieDeclaration(contractNameConstant);
+                foreach(var node in contract.Nodes)
+                {
+                    if (node is StructDefinition structDefn)
+                    {
+                        var structTypedIdent = new BoogieTypedIdent(structDefn.CanonicalName, tnameType);
+                        context.getProgram.AddBoogieDeclaration(new BoogieConstant(structTypedIdent, true));
+                    }
+                }
+            }
+        }
+
+        //Function to build standard global variables for Boogie expressions set.
+        private void buildGlobalVariables()
+        {
+            BoogieTypedIdent balanceId = new BoogieTypedIdent("Balance", new BoogieMapType(BoogieType.Ref, BoogieType.Int));
+            BoogieGlobalVariable balanceVar = new BoogieGlobalVariable(balanceId);
+            context.getProgram.AddBoogieDeclaration(balanceVar);
+
+            BoogieTypedIdent dtypeId = new BoogieTypedIdent("DType", new BoogieMapType(BoogieType.Ref, new BoogieCtorType("ContractName")));
+            BoogieGlobalVariable dtype = new BoogieGlobalVariable(dtypeId);
+            context.getProgram.AddBoogieDeclaration(dtype);
+
+            BoogieTypedIdent addrBalanceId = new BoogieTypedIdent("balance_ADDR", new BoogieMapType(BoogieType.Ref, BoogieType.Int));
+            BoogieGlobalVariable addrBalance = new BoogieGlobalVariable(addrBalanceId);
+            context.getProgram.AddBoogieDeclaration(addrBalance);
+
+            BoogieTypedIdent allocId = new BoogieTypedIdent("Alloc", new BoogieMapType(BoogieType.Ref, BoogieType.Bool));
+            BoogieGlobalVariable alloc = new BoogieGlobalVariable(allocId);
+            context.getProgram.AddBoogieDeclaration(alloc);
+
+            // generate global variables for each array/mapping type to model memory
+            ConstructMemoryVariables();
+
+            BoogieMapType type = new BoogieMapType(BoogieType.Ref, BoogieType.Int);
+            BoogieTypedIdent arrayLengthId = new BoogieTypedIdent("Length", type);
+            BoogieGlobalVariable arrayLength = new BoogieGlobalVariable(arrayLengthId);
+            context.getProgram.AddBoogieDeclaration(arrayLength);
+
+            if (context.TranslateFlags.ModelReverts == true)
+            {
+                BoogieTypedIdent revertId = new BoogieTypedIdent("revert", BoogieType.Bool);
+                BoogieGlobalVariable revert = new BoogieGlobalVariable(revertId);
+                context.getProgram.AddBoogieDeclaration(revert);//
+            }
+
+            if (Flags_HelperClass.InstrumentGas == true)
+            {
+                BoogieTypedIdent gasId = new BoogieTypedIdent("gas", BoogieType.Int);
+                BoogieGlobalVariable gas = new BoogieGlobalVariable(gasId);
+                context.getProgram.AddBoogieDeclaration(gas);
+            }
+        }
+
+
+        //Function to generate struct constructors through iteration of contract definition collection set.
+        private void buildStructConstructor()
+        {
+            foreach (ContractDefinition contract in context.ContractDefinitionsMap)
+            {
+                foreach (var node in contract.Nodes)
+                {
+                    if (node is StructDefinition structDefn)
+                    {
+                        GenerateStructConstructors(contract, structDefn);
+                    }
+                }
+            }
+        }
+
+        private void GenerateStructConstructors(ContractDefinition contract, StructDefinition structDefn)
+        {
+            // generate the internal one without base constructors
+            string procName = structDefn.CanonicalName + "_ctor";
+            List<BoogieVariable> inParams = new List<BoogieVariable>();
+            inParams.AddRange(Conversion_Utility_Tool.GetDefaultInParams());
+            foreach(var member in structDefn.Members)
+            {
+                Debug.Assert(!member.TypeDescriptions.IsStruct(), "Do no handle nested structs yet!");
+                var formalType = Conversion_Utility_Tool.GetBoogieTypeFromSolidityTypeName(member.TypeName);
+                var formalName = member.Name;
+                inParams.Add(new BoogieFormalParam(new BoogieTypedIdent(formalName, formalType)));
+            }
+
+            List<BoogieVariable> outParams = new List<BoogieVariable>();
+            List<BoogieAttribute> attributes = new List<BoogieAttribute>();
+            if (Flags_HelperClass.GenerateInlineAttributes)
+            {
+                attributes.Add(new BoogieAttribute("inline", 1));
+            };
+            BoogieProcedure procedure = new BoogieProcedure(procName, inParams, outParams, attributes);
+            context.getProgram.AddBoogieDeclaration(procedure);
+
+            List<BoogieVariable> localVars = new List<BoogieVariable>();
+            BoogieStmtList procBody = new BoogieStmtList();
+
+            foreach (var member in structDefn.Members)
+            {
+                Debug.Assert(!member.TypeDescriptions.IsStruct(), "Do no handle nested structs yet!");
+                var mapName = member.Name + "_" + structDefn.CanonicalName;
+                var formalName = member.Name;
+                var mapSelectExpr = new BoogieMapSelect(new BoogieIdentifierExpr(mapName), new BoogieIdentifierExpr("this"));
+                procBody.AddStatement(new BoogieAssignCmd(mapSelectExpr, new BoogieIdentifierExpr(member.Name)));
+            }
+
+            BoogieImplementation implementation = new BoogieImplementation(procName, inParams, outParams, localVars, procBody);
+            context.getProgram.AddBoogieDeclaration(implementation);
+        }
+
+
+        private void BuildBoogieRecordType(string typeName, BoogieType btype)
+        {
+
+            // generate the internal one without base constructors
+            string procName = "boogie_si_record_solidity2Boogie_" + typeName;
+            var inVar = new BoogieFormalParam(new BoogieTypedIdent("x", btype));
+            List<BoogieVariable> inParams = new List<BoogieVariable>() { inVar };
+            List<BoogieVariable> outParams = new List<BoogieVariable>();
+
+            BoogieProcedure procedure = new BoogieProcedure(procName, inParams, outParams, null);
+            context.getProgram.AddBoogieDeclaration(procedure);
+        }
+
+        //Generate Fresh Procedure Boogie Type and add as new reference to BoogieProgram
+        private void BuildGlobalProcedureFresh()
+        {
+            // generate the internal one without base constructors
+            string procName = "FreshRefGenerator";
+            List<BoogieVariable> inParams = new List<BoogieVariable>();
+
+            var outVar = new BoogieFormalParam(new BoogieTypedIdent("newRef", BoogieType.Ref));
+            List<BoogieVariable> outParams = new List<BoogieVariable>()
+            {
+                outVar
+            };
+            List<BoogieAttribute> attributes = new List<BoogieAttribute>();
+            if (Flags_HelperClass.GenerateInlineAttributes)
+            {
+                attributes.Add(new BoogieAttribute("inline", 1));
+            };
+            BoogieProcedure procedure = new BoogieProcedure(procName, inParams, outParams, attributes);
+            context.getProgram.AddBoogieDeclaration(procedure);
+
+            List<BoogieVariable> localVars = new List<BoogieVariable>();
+            BoogieStmtList procBody = new BoogieStmtList();
+
+            var outVarIdentifier = new BoogieIdentifierExpr("newRef");
+            BoogieIdentifierExpr allocIdentExpr = new BoogieIdentifierExpr("Alloc");
+            // havoc tmp;
+            procBody.AddStatement(new BoogieHavocCmd(outVarIdentifier));
+            // assume Alloc[tmp] == false;
+            BoogieMapSelect allocMapSelect = new BoogieMapSelect(allocIdentExpr, outVarIdentifier);
+            BoogieExpr allocAssumeExpr = new BoogieBinaryOperation(BoogieBinaryOperation.Opcode.EQ, allocMapSelect, new BoogieLiteralExpr(false));
+            procBody.AddStatement(new BoogieAssumeCmd(allocAssumeExpr));
+            // Alloc[tmp] := true;
+            procBody.AddStatement(new BoogieAssignCmd(allocMapSelect, new BoogieLiteralExpr(true)));
+            // assume tmp != null
+            procBody.AddStatement(new BoogieAssumeCmd(
+                              new BoogieBinaryOperation(BoogieBinaryOperation.Opcode.NEQ, outVarIdentifier, new BoogieIdentifierExpr("null"))));
+
+            BoogieImplementation implementation = new BoogieImplementation(procName, inParams, outParams, localVars, procBody);
+            context.getProgram.AddBoogieDeclaration(implementation);
+        }
+
+        //Function to produce memory allocation as boogie reference types using "alloc"
+        private void GenerateGlobalProcedureAllocMany()
+        {
+            // generate the internal one without base constructors
+            string procName = "HavocAllocMany";
+            List<BoogieVariable> inParams = new List<BoogieVariable>();
+            List<BoogieVariable> outParams = new List<BoogieVariable>();
+            List<BoogieAttribute> attributes = new List<BoogieAttribute>();
+            if (Flags_HelperClass.GenerateInlineAttributes)
+            {
+                attributes.Add(new BoogieAttribute("inline", 1));
+            };
+            BoogieProcedure procedure = new BoogieProcedure(procName, inParams, outParams, attributes);
+            context.getProgram.AddBoogieDeclaration(procedure);
+
+            var oldAlloc = new BoogieLocalVariable(new BoogieTypedIdent("oldAlloc", new BoogieMapType(BoogieType.Ref, BoogieType.Bool)));
+            List<BoogieVariable> localVars = new List<BoogieVariable>() {oldAlloc};
+            
+            BoogieStmtList procBody = new BoogieStmtList();
+            BoogieIdentifierExpr oldAllocIdentExpr = new BoogieIdentifierExpr("oldAlloc");
+            BoogieIdentifierExpr allocIdentExpr = new BoogieIdentifierExpr("Alloc");
+            // oldAlloc = Alloc
+            procBody.AddStatement(new BoogieAssignCmd(oldAllocIdentExpr, allocIdentExpr));            
+            // havoc Alloc
+            procBody.AddStatement(new BoogieHavocCmd(allocIdentExpr));
+
+
+            var qVar = QVarGenerator.NewQVar(0, 0);
+            BoogieMapSelect allocMapSelect = new BoogieMapSelect(allocIdentExpr, qVar);
+            BoogieMapSelect oldAllocMapSelect = new BoogieMapSelect(oldAllocIdentExpr, qVar);
+            BoogieExpr allocAssumeExpr = new BoogieBinaryOperation(BoogieBinaryOperation.Opcode.IMP, oldAllocMapSelect, allocMapSelect);
+            procBody.AddStatement(new BoogieAssumeCmd(new BoogieQuantifiedExpr(true, new List<BoogieIdentifierExpr>() {qVar}, new List<BoogieType>() { BoogieType.Ref }, allocAssumeExpr)));
+
+            BoogieImplementation implementation = new BoogieImplementation(procName, inParams, outParams, localVars, procBody);
+            context.getProgram.AddBoogieDeclaration(implementation);
+        }
+
+
+    
+        //Function to construct memory variables for ArrayMap.keys and Mapping Frame
+        private void ConstructMemoryVariables()
+        {
+            HashSet<KeyValuePair<BoogieType, BoogieType>> generatedTypes = new HashSet<KeyValuePair<BoogieType, BoogieType>>();
+            // mappings
+            foreach (ContractDefinition contract in context.MappingFrame.Keys)
+            {
+                foreach (VariableDeclaration variableDeclaration in context.MappingFrame[contract])
+                {
+                    //Iteratve over MappingFrame and generate keys 
+                    Debug.Assert(variableDeclaration.TypeName is Mapping);
+                    Mapping mapping = variableDeclaration.TypeName as Mapping;
+                    ConstructMappingMemoryArray(mapping, generatedTypes);
+                }
+            }
+            //Iterate over array maps and construct appropriate memory maps from this.
+            foreach (ContractDefinition contract in context.constructArrayMaps.Keys)
+            {
+                foreach (VariableDeclaration variableDeclaration in context.constructArrayMaps[contract])
+                {
+                    Debug.Assert(variableDeclaration.TypeName is ArrayTypeName);
+                    ArrayTypeName array = variableDeclaration.TypeName as ArrayTypeName;
+                    ConstructArrayMemoryMap(array, generatedTypes);
+                }
+            }
+        }
+
+        //Construct Memory Maps for Arrays for Mapping and ArrayTypeName types.
+        private void ConstructMappingMemoryArray(Mapping mapping, HashSet<KeyValuePair<BoogieType, BoogieType>> generatedTypes)
+        {
+            BoogieType boogieKeyType = Conversion_Utility_Tool.GetBoogieTypeFromSolidityTypeName(mapping.KeyType);
+            BoogieType boogieValueType = null;
+            if (mapping.ValueType is Mapping submapping)
+            {
+                boogieValueType = BoogieType.Ref;
+                ConstructMappingMemoryArray(submapping, generatedTypes);
+            }
+            else if (mapping.ValueType is ArrayTypeName array)
+            {
+                boogieValueType = BoogieType.Ref;
+                ConstructArrayMemoryMap(array, generatedTypes);
+            }
+            else { boogieValueType = Conversion_Utility_Tool.GetBoogieTypeFromSolidityTypeName(mapping.ValueType); }
+
+            KeyValuePair<BoogieType, BoogieType> pair = new KeyValuePair<BoogieType,BoogieType>(boogieKeyType, boogieValueType);
+            if (!generatedTypes.Contains(pair))
+            {
+                generatedTypes.Add(pair);
+                BuildSingleMapMemoryName(boogieKeyType, boogieValueType);
+            }
+        }
+
+        //Build Memory Map for Array types, 
+        private void ConstructArrayMemoryMap(ArrayTypeName array, HashSet<KeyValuePair<BoogieType, BoogieType>> generatedTypes)
+        {
+            BoogieType boogieKeyType = BoogieType.Int;
+            BoogieType boogieValueType = null;
+            if (array.BaseType is ArrayTypeName subarray)
+            {
+                boogieValueType = BoogieType.Ref;
+                ConstructArrayMemoryMap(subarray, generatedTypes); //construct array memory map with sub array
+            }
+            else if (array.BaseType is Mapping mapping)
+            {
+                boogieValueType = BoogieType.Ref;
+                ConstructMappingMemoryArray(mapping, generatedTypes); // construct array memory map using mapping type
+            }
+            else {
+                boogieValueType = Conversion_Utility_Tool.GetBoogieTypeFromSolidityTypeName(array.BaseType); //type cannot be resolve, request type declaration 
+            }
+
+            KeyValuePair<BoogieType, BoogieType> pair = new KeyValuePair<BoogieType, BoogieType>(boogieKeyType, boogieValueType);
+            if (generatedTypes.Contains(pair) == false)
+            {
+                generatedTypes.Add(pair);
+                BuildSingleMapMemoryName(boogieKeyType, boogieValueType);
+            }
+        }
+
+        //Build Single Memory Map using key and value types
+        private void BuildSingleMapMemoryName(BoogieType keyTypes, BoogieType valueTypes)
+        {
+            BoogieMapType map = new BoogieMapType(keyTypes, valueTypes);
+            map = new BoogieMapType(BoogieType.Ref, map);
+
+            string name = Flags_HelperClass.generateMemoryMapName(keyTypes, valueTypes);
+            context.getProgram.AddBoogieDeclaration(new BoogieGlobalVariable(new BoogieTypedIdent(name, map)));
+        }
+    }
+}
