Sources/ConversionToBoogie/accumulator_SOL_Contract.cs
@@ -5,21 +5,22 @@ namespace ConversionToBoogie
     using Sol_Syntax_Tree;
 
     /**
-     * accumulaltor function to handle adding contract definition node to overall translator context
+     * accumulator function to handle adding contract definition node to overall translator context
      */
     public class accumulator_SOL_Contract : Generic_Syntax_Tree_Visitor
     {
-        private TranslatorContext classTranslatorContext;
+        private AST_Handler classTranslatorContext;
 
-        public override bool ContractDefinition_VisitNode(ContractDefinition currentNode)
+        public override bool ContractDefinition_ReTraceNode(ContractDefinition currentNode)
         {
+            //if reference type is not equal to null then add contract to ASTH refrence
             if(classTranslatorContext != null)
-                classTranslatorContext.AddContract(currentNode);
+                classTranslatorContext.InsertContractInMapping(currentNode);
             return false;
         }
 
         //provides base context, called after instantiation
-        public void setContext(TranslatorContext tempContext)
+        public void setContext(AST_Handler tempContext)
         {
             this.classTranslatorContext = tempContext;
         }
