UnitTests/DAO-demo.sol
@@ -2,7 +2,6 @@ pragma solidity >=0.4.24<0.6.0;
 
 import "C:/OversightRepo/Oversight/Project/UnitTests/ValidationSpecs.sol";
 
-
 contract SimpleDAO {
     mapping (address => uint) public credit;
 
